More ordinal stuff+cleanup, and other small improvements

Isabelle_Set/Ordinal.thy
@@ -5,52 +5,65 @@ imports Subset
 
 begin
 
-definition Ord :: \<open>set type\<close> where [typedef]:
+text \<open>
+  The class of ordinal numbers is defined abstractly, as the \<in>-transitive sets
+  whose members are also \<in>-transitive.
+\<close>
+
+definition [typedef]:
   "Ord \<equiv> type (\<lambda>x. mem_transitive x \<and> (\<forall>y \<in> x. mem_transitive y))"
 
-lemma emptyset_Ord [intro!]: "{} : Ord"
-  by unfold_types auto
+lemma OrdI:
+  "mem_transitive X \<Longrightarrow> (\<And>x. x \<in> X \<Longrightarrow> mem_transitive x) \<Longrightarrow> X: Ord"
+  unfolding Ord_def by (auto simp: has_type_type)
 
-lemma Ord_transitive [elim]: "x : Ord \<Longrightarrow> y \<in> x \<Longrightarrow> y : Ord"
+text \<open>Basic properties of ordinals:\<close>
+
+lemma Ord_mem_closed [elim]: "x : Ord \<Longrightarrow> y \<in> x \<Longrightarrow> y : Ord"
   by unfold_types (fastforce simp: mem_transitive_def)
 
-lemma Ord_elem_subset: "x : Ord \<Longrightarrow> y \<in> x \<Longrightarrow> y \<subseteq> x"
+lemma Ord_mem_transitive:
+  "x: Ord \<Longrightarrow> mem_transitive x"
+  by unfold_types
+
+lemma Ord_mem_transitive' [elim]: "x : Ord \<Longrightarrow> y \<in> x \<Longrightarrow> y \<subseteq> x"
   by unfold_types (fastforce simp: mem_transitive_def)
+
+lemma [derive]: "x: Ord \<Longrightarrow> y: element x \<Longrightarrow> y: subset x"
+  by (fold element_type_iff subset_type_iff) (fact Ord_mem_transitive')
 
 (*Adapted from a proof by Chad Brown*)
 lemma Ord_trichotomy_aux:
   "X : Ord \<Longrightarrow> Y : Ord \<Longrightarrow> X \<notin> Y \<Longrightarrow> Y \<notin> X \<Longrightarrow> X = Y"
 proof (induction X Y rule: mem_double_induct)
   fix X Y
-  assume ord: "X : Ord" "Y : Ord"
-  assume IH1: "\<And>x. x \<in> X \<Longrightarrow> x : Ord \<Longrightarrow> Y : Ord \<Longrightarrow> x \<notin> Y \<Longrightarrow> Y \<notin> x \<Longrightarrow> x = Y"
-  assume IH2: "\<And>y. y \<in> Y \<Longrightarrow> X : Ord \<Longrightarrow> y : Ord \<Longrightarrow> X \<notin> y \<Longrightarrow> y \<notin> X \<Longrightarrow> X = y"
-  assume *: "X \<notin> Y" "Y \<notin> X"
+  assume
+    ord: "X : Ord" "Y : Ord" and
+    IH1: "\<And>x. x \<in> X \<Longrightarrow> x : Ord \<Longrightarrow> Y : Ord \<Longrightarrow> x \<notin> Y \<Longrightarrow> Y \<notin> x \<Longrightarrow> x = Y" and
+    IH2: "\<And>y. y \<in> Y \<Longrightarrow> X : Ord \<Longrightarrow> y : Ord \<Longrightarrow> X \<notin> y \<Longrightarrow> y \<notin> X \<Longrightarrow> X = y" and
+    *: "X \<notin> Y" "Y \<notin> X"
   show "X = Y"
-  proof (rule extensionality)
-    show "X \<subseteq> Y"
-    proof
-      fix x assume "x \<in> X"
-      with ord have "x \<subseteq> X" "x : Ord" by (auto elim!: Ord_elem_subset)
-      with * ord IH1 \<open>x \<in> X\<close> show "x \<in> Y" by blast
-    qed
-    show "Y \<subseteq> X"
-    proof
-      fix y assume "y \<in> Y"
-      with ord have "y \<subseteq> Y" "y : Ord" by (auto elim!: Ord_elem_subset)
-      with * ord IH2 \<open>y \<in> Y\<close> show "y \<in> X" by blast
-    qed
+  proof (rule equalityI)
+    fix x assume "x \<in> X"
+    with ord have "x \<subseteq> X" "x : Ord" by (auto elim!: Ord_mem_transitive')
+    with * ord IH1 \<open>x \<in> X\<close> show "x \<in> Y" by blast
+  next
+    fix y assume "y \<in> Y"
+    with ord have "y \<subseteq> Y" "y : Ord" by (auto elim!: Ord_mem_transitive')
+    with * ord IH2 \<open>y \<in> Y\<close> show "y \<in> X" by blast
   qed
 qed
 
-lemma Ord_trichotomy: "\<lbrakk>X : Ord; Y : Ord\<rbrakk> \<Longrightarrow> X \<in> Y \<or> X = Y \<or> Y \<in> X"
-  using Ord_trichotomy_aux by blast
+lemma Ord_trichotomy: "\<lbrakk>X: Ord; Y: Ord\<rbrakk> \<Longrightarrow> X \<in> Y \<or> X = Y \<or> Y \<in> X"
+  using Ord_trichotomy_aux by auto
+
+lemma emptyset_Ord [type]: "{} : Ord"
+  by unfold_types auto
 
 
-section \<open>The von Neumann ordinals\<close>
+section \<open>Successor ordinals\<close>
 
-definition succ :: "set \<Rightarrow> set"
-  where "succ x \<equiv> x \<union> {x}"
+definition "succ x \<equiv> x \<union> {x}"
 
 lemma succ_Ord: "x : Ord \<Longrightarrow> succ x : Ord"
   unfolding succ_def by unfold_types (fastforce simp: mem_transitive_def)
@@ -62,13 +75,13 @@ proof (rule, elim equalityE)
   thus False using mem_irrefl by auto
 qed
 
-lemma succ_mem: "x \<in> succ x"
+lemma succ_mem [simp]: "x \<in> succ x"
   unfolding succ_def by auto
 
-lemma succ_memI: "x \<in> y \<Longrightarrow> x \<in> succ y"
+lemma succ_memI [simp]: "x \<in> y \<Longrightarrow> x \<in> succ y"
   unfolding succ_def by auto
 
-lemma succ_not_empty [simp]: "succ n \<noteq> {}"
+lemma succ_not_empty [simp]: "succ x \<noteq> {}"
   unfolding succ_def by auto
 
 lemmas empty_not_succ = succ_not_empty[symmetric, simp]
@@ -77,21 +90,20 @@ lemmas
   succ_emptyE = notE[OF succ_not_empty] and
   empty_succE = notE[OF empty_not_succ]
 
-
-lemma succ_inject [dest]: "succ n = succ m \<Longrightarrow> n = m"
+lemma succ_inject [dest]: "succ x = succ y \<Longrightarrow> x = y"
 proof (rule ccontr)
-  assume succ_eq: "succ n = succ m"
-  assume neq: "n \<noteq> m"
+  assume succ_eq: "succ x = succ y"
+  assume neq: "x \<noteq> y"
 
-  have "n \<in> succ n" unfolding succ_def by blast
-  with succ_eq have "n \<in> succ m" by simp
-  with neq have "n \<in> m" unfolding succ_def by blast
+  have "x \<in> succ x" unfolding succ_def by blast
+  with succ_eq have "x \<in> succ y" by simp
+  with neq have "x \<in> y" unfolding succ_def by blast
 
-  have "m \<in> succ m" unfolding succ_def by blast
-  with succ_eq have "m \<in> succ n" by simp
-  with neq have "m \<in> n" unfolding succ_def by blast
+  have "y \<in> succ y" unfolding succ_def by blast
+  with succ_eq have "y \<in> succ x" by simp
+  with neq have "y \<in> x" unfolding succ_def by blast
 
-  from \<open>n \<in> m\<close> \<open>m \<in> n\<close> show False using mem_asym by blast
+  from \<open>x \<in> y\<close> \<open>y \<in> x\<close> show False using mem_asym by blast
 qed
 
 lemma Univ_succ_closed [intro]: "x \<in> Univ X \<Longrightarrow> succ x \<in> Univ X"
@@ -148,16 +160,40 @@ proof (induction rule: omega_induct)
     thus "{} \<in> succ (succ n)" unfolding succ_def by auto
 qed
 
-lemma omega_pred_exists [rule_format]:
+(*Characterizes the elements of \<omega> as {} or succ n for some n \<in> \<omega>*)
+lemma omega_elems [rule_format]:
   "n \<in> \<omega> \<Longrightarrow> n \<noteq> {} \<longrightarrow> (\<exists>!m\<in> \<omega>. n = succ m)"
   by (erule omega_cases) auto
 
-text \<open>Truncated predecessor function:\<close>
+lemma omega_Ord: "\<omega>: Ord"
+proof (rule OrdI, unfold mem_transitive_def; rule allI, rule impI)
+  fix x assume "x \<in> \<omega>"
+  thus "x \<subseteq> \<omega>"
+    by (induction x rule: omega_induct) (auto simp: succ_def)
+
+  fix y assume "y \<in> x"
+  with \<open>x \<in> \<omega>\<close> show "y \<subseteq> x"
+    by (induction x rule: omega_induct) (auto simp: succ_def)
+qed
+
+lemma omega_elem_Ord: "n \<in> \<omega> \<Longrightarrow> n: Ord"
+  using omega_Ord Ord_mem_closed by auto
+
+lemma [derive]: "n: element \<omega> \<Longrightarrow> n: Ord"
+  by (fold element_type_iff) (fact omega_elem_Ord)
+
+lemma omega_elem_mem_transitive: "n \<in> \<omega> \<Longrightarrow> mem_transitive n"
+  using omega_elem_Ord Ord_mem_transitive by auto
+
+lemma omega_elem_subset: "n \<in> \<omega> \<Longrightarrow> n \<subseteq> \<omega>"
+  using omega_Ord Ord_mem_transitive' by auto
+
+text \<open>Truncated predecessor function\<close>
 
 definition "pred n = (if n = {} then {} else (THE m \<in> \<omega>. n = succ m))"
 
 lemma pred_omega [simp]: "n \<in> \<omega> \<Longrightarrow> pred n \<in> \<omega>"
-  unfolding pred_def by (auto intro: BTheI1 omega_pred_exists)
+  unfolding pred_def by (auto intro: BTheI1 omega_elems)
 
 lemma pred_empty [simp]: "pred {} = {}"
   unfolding pred_def by auto
@@ -166,7 +202,7 @@ lemma pred_succ [simp]: "n \<in> \<omega> \<Longrightarrow> pred (succ n) = n"
   unfolding pred_def by auto
 
 lemma succ_pred [simp]: "\<lbrakk>n \<in> \<omega>; n \<noteq> {}\<rbrakk> \<Longrightarrow> succ (pred n) = n"
-  unfolding pred_def by (simp, rule sym, rule BTheI2) (fact omega_pred_exists)
+  unfolding pred_def by (simp, rule sym, rule BTheI2) (fact omega_elems)
 
 
 end
